PastaLean/PyGens/test.lean
@@ -45,4 +45,4 @@ def factorial'rn := fun (n : Int) ↦
       return result)
 
 
-#eval factorial'rn 10
+-- #eval factorial'rn 10
